Call some additional string functions

hello.fst
@@ -1,20 +1,42 @@
 module Hello
 open FStar.IO
 open FStar.ST
+open FStar.String
+open FStar.List
 
-let state = ST.alloc 0
+val buffer : ref (list (ref string))
+let buffer = ST.alloc [ST.alloc ""]
+let cursor_row = ST.alloc 0
+let cursor_col = ST.alloc 0
+
+val str_insert : int -> char -> string -> string
+let str_insert i ch str = strcat (substring str 0 i) (strcat (make 1 ch) (substring str i (strlen str - i)))
+
+val insert_char : char -> ML unit
+let insert_char ch =
+  let sref = nth !buffer !cursor_row in
+  let str = str_insert !cursor_col ch !sref in
+  sref := str
+
+val print_lines : list (ref string) -> ML unit
+let rec print_lines rs' = match rs' with
+  | [] -> ()
+  | (r::rs) -> print_string !r; print_string "\n"; print_lines rs
+
+val print_buffer : unit -> ML unit
+let print_buffer () =
+  print_lines !buffer
+
+val handle_key : char -> ML unit
+let handle_key ch =
+  insert_char ch
 
 val editor : unit -> ML unit
 let rec editor () =
-  print_int !state;
   let ch = input_char () in
-  (if ch = 'a' then
-    state := !state + 1
-  else
-    state := !state - 1);
+  handle_key ch;
+  print_buffer ();
   editor ()
 ;;
    
 editor ()
-
-
