Makefile
@@ -2,10 +2,13 @@ LIB=$(FSTAR_HOME)/lib
 BIN=$(FSTAR_HOME)/bin
 FSTAR=$(BIN)/fstar.exe
 
+ADMIT=--admit_fsi FStar.Set --admit_fsi FStar.Heap --admit_fsi FStar.ST --admit_fsi FStar.All --admit_fsi FStar.IO
+LIBFILES=set.fsi heap.fst st.fst all.fst io.fsti string.fst list.fst
+
 ocaml: out hello.fst
-	$(FSTAR) --odir out --codegen OCaml hello.fst
-	cp $(LIB)/ml/prims.ml $(LIB)/ml/FStar_IO.ml $(LIB)/ml/FStar_ST.ml out
-	(cd out; ocamlc -o hello.exe prims.ml FStar_IO.ml FStar_ST.ml Hello.ml)
+	$(FSTAR) --debug hello.fst --odir out --codegen OCaml $(ADMIT) $(LIBFILES) hello.fst
+	cp $(LIB)/ml/prims.ml $(LIB)/ml/FStar_IO.ml $(LIB)/ml/FStar_ST.ml $(LIB)/ml/FStar_String.ml $(LIB)/ml/FStar_List.ml out
+	(cd out; ocamlfind ocamlc -o hello.exe -package batteries -linkpkg prims.ml FStar_IO.ml FStar_ST.ml FStar_List.ml FStar_String.ml Hello.ml)
 	stty -echo -icanon
 	./out/hello.exe
 	stty echo icanon
